\documentclass[10pt]{article}

\usepackage{amsmath, amsfonts, bm}
\usepackage[margin=1in]{geometry}

\input{../../latex_inputs/math_commands.tex}

\begin{document}

\title{Notes: Moment Generating Functions}
\author{Aiden Kenny}
\maketitle

\section{Introduction}

[Fill out later]

\section{Multiple random variables}

Suppose we have a group of \( n \) independent random variables \( X_i \), \( i \in [n] \),
which gives us
\( \rVector{X} = [X_1, \ldots, X_n]^{\top} \).
Each random variable also has a well-defined moment generating function \( M_{X_i}(t) \).

\vspace*{2em}\noindent
\textbf{Linear combinations}:
Let
\begin{align*}
    S(\rVector{X})
    = \beta_0 + \mVector{\beta}^\top \rVector{X}
    = \beta_0 + \sum_{i=1}^n \beta_i X_i
\end{align*}
be a linear combination of the random variables in \( \rVector{X} \).
Then it's moment generating function is given by
\begin{align}
    M_{S(\rVector{X})}(t)
    = \mathrm{e}^{\beta_0} \prod_{i=1}^n M_{X_i}(\beta_i t).
\end{align}
The m.g.f. is given as
\begin{align*}
    M_{S(\rVector{X})}(t)
    = \ev\Big[ \exp(t S) \Big]
    % = \ev \left[ \exp \left( t \beta_0 + \sum_{i = 1}^n t \beta_i X_i \right) \right]
    = \int_{\mathcal{D}_{S(\rVector{X})}}
    \exp(t S)
    \, f_{\rVector{X}}(\mVector{x})
    \, \mathrm{d}\mVector{x}.
\end{align*}
Because it is exponentiation,
we can write
\begin{align*}
    \exp(t S)
    = \exp \left( t \beta_0 + \sum_{i = 1}^n t \beta_i X_i \right)
    = \exp(t \beta_0) \prod_{i=1}^{n} \exp(t \beta_i X_i),
\end{align*}
and because each r.v. is independent, we can write
\begin{align*}
    f_{\rVector{X}}(\mVector{x})
    = \prod_{i=1}^{n} f_{X_i}(x_i).
\end{align*}
Substituting these in and re-arranging gives
\begin{align*}
    M_{S(\rVector{X})}(t)
    &= \int_{\mathcal{D}_{S(\rVector{X})}}
    \exp(t S)
    \, f_{\rVector{X}}(\mVector{x})
    \, \mathrm{d}\mVector{x}
    = \int_{\mathcal{D}_{X_1}} \cdots \int_{\mathcal{D}_{X_n}}
    \exp(t \beta_0) \prod_{i=1}^{n} \exp(t \beta_i X_i)
    \prod_{i=1}^{n} f_{X_i}(x_i)
    \, \mathrm{d}x_1
    \cdots
    \, \mathrm{d}x_n \\
    &= \exp(t \beta_0)
    \prod_{i=1}^{n}
    \int_{\mathcal{D}_{X_i}}
    \exp(t \beta_i X_i)
    f_{X_i}(x_i)
    \, \mathrm{d}x_i
    = \exp(t \beta_0)
    \prod_{i=1}^{n}
    M_{X_i}(t \beta_i).
\end{align*}

\end{document}